begin working to use wp_ReadSlice

example/calendar_proof.v
@@ -7,6 +7,7 @@ From Perennial.goose_lang Require Import lib.slice.pred_slice.
 Module Calendar.
   Section Calendar.
 
+    Typeclasses Opaque app.
     Context `{!heapGS Σ}.
 
     Record C :=
@@ -16,7 +17,7 @@ Module Calendar.
 
     Fixpoint has_events_encoding (encoding:list u8) (events: list Event.C) : Prop :=
       match events with
-      | [] => True
+      | [] => encoding = []
       | e :: tail => ∃ (e_enc tail_enc:list u8), encoding = e_enc ++ tail_enc /\
                                                Event.has_encoding e_enc e /\
                                                has_events_encoding tail_enc tail
@@ -30,9 +31,82 @@ Module Calendar.
     Definition own (args__v : val) (args__c : C) (dq :dfrac) : iProp Σ :=
       ∃ (events__sl : Slice.t),
         "%Hown_struct" ∷ ⌜ args__v = ((slice_val events__sl), #())%V ⌝ ∗
-        (* FIXME: That `ty' is wrong. How to I get an EventT? *)
-        "Hown_events" ∷ is_pred_slice Event.own events__sl byteT dq args__c.(events).
+        "Hown_events" ∷ is_pred_slice Event.own events__sl (struct.t Event)
+          dq args__c.(events).
+
+    Lemma wp_Encode (args__v : val) (args__c : C) (prefix : list u8) (pre_sl : Slice.t) (dq: dfrac) :
+      {{{
+            own args__v args__c dq ∗
+            own_slice pre_sl byteT (DfracOwn 1) prefix
+      }}}
+        MarshalCalendar args__v (slice_val pre_sl)
+      {{{
+            enc enc_sl, RET (slice_val enc_sl);
+            ⌜ has_encoding enc args__c ⌝ ∗
+            own_slice enc_sl byteT (DfracOwn 1) (prefix ++ enc) ∗
+            own args__v args__c dq
+      }}}.
+    Proof.
+      iIntros (?) "[Hown Hsl] HΦ".
+      wp_rec. wp_pures.
+      iUnfold own in "Hown". iNamed "Hown". rewrite Hown_struct.
+      iUnfold is_pred_slice in "Hown_events".
+      iDestruct "Hown_events" as "[%es [Hown_events #HΨ_events]]".
+      iDestruct (big_sepL2_length with "HΨ_events") as "%HΨ_events_len".
+      wp_apply (wp_ref_to); first by val_ty.
+      iIntros (?) "Hptr". wp_pures.
     
+      wp_apply (wp_slice_len).
+      iDestruct (own_slice_small_sz with "Hown_events") as "%Hargs_events_sz".
+      wp_load. wp_apply (wp_WriteInt with "[$Hsl]").
+      iIntros (?) "Hsl". wp_store. wp_pures.
+      
+      (* TODO: Finish once wp_WriteSlice exists *)
+    Admitted.
+    
+    Lemma wp_Decode (enc : list u8) (enc_sl : Slice.t) (args__c : C) (suffix : list u8) (dq : dfrac) :
+      {{{
+            ⌜ has_encoding enc args__c ⌝ ∗
+            own_slice_small enc_sl byteT dq (enc ++ suffix)
+      }}}
+        UnmarshalCalendar (slice_val enc_sl)
+      {{{
+            args__v suff_sl, RET (args__v, suff_sl);
+            own args__v args__c (DfracOwn 1) ∗
+            own_slice_small suff_sl byteT dq suffix
+      }}}.
+    Proof.
+      iIntros (?) "[%Henc Hsl] HΦ". wp_rec.
+      wp_apply wp_ref_to; first done.
+      iIntros (l__s) "Hs". wp_pures.
+      
+      wp_apply wp_ref_of_zero; first done.
+      iIntros (l__events) "Hevents". wp_pures.
+
+      wp_apply wp_ref_of_zero; first done.
+      iIntros (l__eventsLen) "HeventsLen". wp_pures.
+
+      destruct Henc as [events_enc [Henc Henc_events]].
+      rewrite Henc. rewrite -?app_assoc.
+
+      wp_load. wp_apply (wp_ReadInt with "[$Hsl]").
+      iIntros (?) "Hsl". wp_pures. wp_store. wp_store.
+
+      wp_load. wp_load.
+      
+      wp_apply (wp_ReadSlice _ _ args__c.(events) _ Event.has_encoding Event.own with "[]").
+      {
+        iIntros (???) "Hown". iUnfold Event.own in "Hown".
+        iUnfold timestamp_proof.TimeStamp.own in "Hown".
+        iDestruct "Hown" as "[%stv [%etv Hown]]".
+        iNamed "Hown".
+        iNamed "Hown_startTime".
+        iNamed "Hown_endTime".
+        iPureIntro.
+        rewrite Hown_struct.
+        rewrite Hown_struct0.
+        rewrite Hown_struct1.
+      } { done. }
   End Calendar.
 End Calendar.
     
